Make the Curve25519 call-graph indexed over a predicate
Instead of being parameterized over a field representation, the generic
code is now parameterized over a field representation and a global
invariant.

```
type field_spec = M51 | M64
let index = field_spec & Type
```

Therefore, at instantiation-time, we now do:

```
let scalarmult_vale64 = mk_scalarmult (M64, Vale.CPU_Features.(adx /\ bmi2))
let scalarmult_hacl64 = mk_scalarmult (M64, True)
let scalarmult_hacl51 = mk_scalarmult (M51, True)
```

where `mk_scalarmult` is the higher-order, tactic-rewritten function
that generates a specialized instance of `scalarmult` for:
- a given field representation
- a global invariant that is carried throughout the whole call-graph
- a given set of functions that require the global invariant and
  implement the core operations for that field representation.

M64 has two implementations; M51 only has one. This is modular: further
implementations possibly requiring new fancy invariants may be added at
any time without having to touch the curve implementation.

This fixes a previous limitation of the curve code, wherein the hacl64
version would still inherit the Vale precondition because the code had
no way of referring to an abstract precondition that would be
instantiated depending on what the core operations need.

The implementation works and has the nice property that it didn't
require modifying the tactic. However, the result is somewhat verbose,
and achieving proper reduction behavior was a struggle. Indeed, having
the index be a pair now requires us to be very careful when destructing
and/or constructing.

1) In types, intermediary let-bindings where the left-hand side is a
pattern block reduction and prevent calls from type-checking. Therefore,
we do:

```
inline_for_extraction
let f_t (i: index) =
  let s = fst i in
  let p = snd i in
  ... ->
  felem s ->
  ... ->
  Stack (fun _ -> requires p /\ ...) (...)
```

instead of `let s, p = i`.

2) The default `fst` projector is not marked as `inline_for_extraction`,
so we shadow it and only use our version marked as
inline_for_extraction. In code, we use `[@inline_let]` to define `s`.

3) The presence of a pair seems to block reduction. This does not work:

```
inline_for_extraction
let i = M51, True

val f: #i:index -> f_t i
```

but this does:

```
val f: #i:index -> f_t (M51, True)
```.

4) The index being a pair seems to interact poorly with implicit
argument inference and many call-sites had to be annotated explicitly.

5) Unless the predicate is annotated at Type0, universe binding problems
arise, as the tactic assumes that the code being rewritten is not
universe-polymorphic.

--------------------------------------------------------------------------------

There may be other solutions; for instance, one might imagine a second
index that is not touched by the tactic, e.g:

```
val g_t (s: field_spec) =
  #p:Type ->
  ... ->
  felem s ->
  ... ->
  Stack (fun _ -> requires p /\ ...) ...

val g: #s:field_spec -> g_t s
```

This is only marginally more verbose than the solution in this commit;
it might also reduce struggles when it comes to dealing with pairs.
However, the implicit argument will have to be explicitly provided,
unless...

... unless we write a tactic to infer `p` by just doing a lookup in the
context and finding a `p` that is an argument to the current function,
and has type `Type`. But this is also high-tech and we may have blown
the complexity budget for that.

code/curve25519/Hacl.Impl.Curve25519.AddAndDouble.fst
@@ -50,14 +50,16 @@ let point_post_add_t #s h f =
   | M64 -> True
 
 val point_add_and_double0:
-    #s:field_spec
-  -> nq_p1:point s
+    #i:index -> (
+  let s = fst i in
+  let p = snd i in
+    nq_p1:point s
   -> ab:lbuffer (limb s) (2ul *! nlimb s)
   -> dc:lbuffer (limb s) (2ul *! nlimb s)
   -> tmp2:felem_wide2 s
   -> Stack unit
     (requires fun h0 ->
-      (s = M64 ==> Vale.X64.CPU_Features_s.(adx_enabled /\ bmi2_enabled)) /\
+      p /\
       live h0 nq_p1 /\ live h0 ab /\ live h0 dc /\ live h0 tmp2 /\
       disjoint nq_p1 ab /\ disjoint nq_p1 dc /\ disjoint nq_p1 tmp2 /\
       disjoint ab dc /\ disjoint ab tmp2 /\ disjoint dc tmp2 /\
@@ -67,9 +69,11 @@ val point_add_and_double0:
     (ensures  fun h0 _ h1 ->
       modifies (loc nq_p1 |+| loc dc |+| loc tmp2) h0 h1 /\
       point_post_add_t h1 (get_x nq_p1) /\ point_post_sub_t h1 (get_z nq_p1) /\
-      fget_xz h1 nq_p1 == S.add_and_double1_0 (fget_x h0 ab) (fget_z h0 ab) (fget_xz h0 nq_p1))
+      fget_xz h1 nq_p1 == S.add_and_double1_0 (fget_x h0 ab) (fget_z h0 ab) (fget_xz h0 nq_p1)))
 [@ Meta.Attribute.inline_ ]
-let point_add_and_double0 #s nq_p1 ab dc tmp2 =
+let point_add_and_double0 #i nq_p1 ab dc tmp2 =
+  [@inline_let]
+  let s, _ = i in
   let x3 = sub nq_p1 0ul (nlimb s) in
   let z3 = sub nq_p1 (nlimb s) (nlimb s) in
   let a : felem s = sub ab 0ul (nlimb s) in
@@ -88,14 +92,16 @@ let point_add_and_double0 #s nq_p1 ab dc tmp2 =
   fsub z3 d c  // z3 = da - cb
 
 val point_add_and_double1:
-    #s:field_spec
-  -> nq:point s
+    #i:index -> (
+  let s = fst i in
+  let p = snd i in
+    nq:point s
   -> nq_p1:point s
   -> tmp1:lbuffer (limb s) (4ul *! nlimb s)
   -> tmp2:felem_wide2 s
   -> Stack unit
     (requires fun h0 ->
-      (s = M64 ==> Vale.X64.CPU_Features_s.(adx_enabled /\ bmi2_enabled)) /\
+      p /\
       live h0 nq /\ live h0 nq_p1 /\ live h0 tmp1 /\ live h0 tmp2 /\
       disjoint nq nq_p1 /\ disjoint nq tmp1 /\ disjoint nq tmp2 /\
       disjoint nq_p1 tmp1 /\ disjoint nq_p1 tmp2 /\ disjoint tmp1 tmp2 /\
@@ -109,9 +115,11 @@ val point_add_and_double1:
       state_inv_t h1 (get_x nq_p1) /\ state_inv_t h1 (get_z nq_p1) /\
       (fget_xz h1 nq, fget_xz h1 nq_p1) ==
 	S.add_and_double1_1 (feval h0 (gsub tmp1 0ul (nlimb s)))
-	  (feval h0 (gsub tmp1 (nlimb s) (nlimb s))) (fget_xz h0 nq_p1))
+	  (feval h0 (gsub tmp1 (nlimb s) (nlimb s))) (fget_xz h0 nq_p1)))
 [@ Meta.Attribute.inline_ ]
-let point_add_and_double1 #s nq nq_p1 tmp1 tmp2 =
+let point_add_and_double1 #i nq nq_p1 tmp1 tmp2 =
+  [@inline_let]
+  let s, _ = i in
   let x2 = sub nq 0ul (nlimb s) in
   let z2 = sub nq (nlimb s) (nlimb s) in
   let x3 = sub nq_p1 0ul (nlimb s) in
@@ -134,10 +142,10 @@ let point_add_and_double1 #s nq nq_p1 tmp1 tmp2 =
   fsqr2 nq_p1 nq_p1 tmp2;   // x3|z3 = x3*x3|z3*z3
 
   copy_felem a c;                           // a = bb
-  fsub c d c;   // c = e = aa - bb
+  fsub #i c d c;   // c = e = aa - bb
   assert_norm (121665 < pow2 17);
-  fmul1 b c (u64 121665); // b = e * 121665
-  fadd b b d;   // b = (e * 121665) + aa
+  fmul1 #i b c (u64 121665); // b = e * 121665
+  fadd #i b b d;   // b = (e * 121665) + aa
 
   (* CAN RUN IN PARALLEL *)
   //fmul x2 d a;  // x2 = aa * bb
@@ -145,21 +153,22 @@ let point_add_and_double1 #s nq nq_p1 tmp1 tmp2 =
   fmul2 nq dc ab tmp2  // x2|z2 = aa * bb | e * (aa + (e * 121665))
 
 val point_add_and_double:
-    #s:field_spec
-  -> q:point s
+    #i:index -> (
+  let s = fst i in
+  let p = snd i in
+    q:point s
   -> p01_tmp1:lbuffer (limb s) (8ul *! nlimb s)
   -> tmp2:felem_wide2 s
   -> Stack unit
     (requires fun h0 ->
-      (s = M64 ==> Vale.X64.CPU_Features_s.(adx_enabled /\ bmi2_enabled)) /\
-    (
       let nq = gsub p01_tmp1 0ul (2ul *! nlimb s) in
       let nq_p1 = gsub p01_tmp1 (2ul *! nlimb s) (2ul *! nlimb s) in
+      p /\
       live h0 q /\ live h0 p01_tmp1 /\ live h0 tmp2 /\
       disjoint q p01_tmp1 /\ disjoint q tmp2 /\ disjoint p01_tmp1 tmp2 /\
       state_inv_t h0 (get_x q) /\ state_inv_t h0 (get_z q) /\
       state_inv_t h0 (get_x nq) /\ state_inv_t h0 (get_z nq) /\
-      state_inv_t h0 (get_x nq_p1) /\ state_inv_t h0 (get_z nq_p1)))
+      state_inv_t h0 (get_x nq_p1) /\ state_inv_t h0 (get_z nq_p1))
     (ensures  fun h0 _ h1 -> (
       let nq = gsub p01_tmp1 0ul (2ul *! nlimb s) in
       let nq_p1 = gsub p01_tmp1 (2ul *! nlimb s) (2ul *! nlimb s) in
@@ -167,9 +176,12 @@ val point_add_and_double:
       state_inv_t h1 (get_x nq) /\ state_inv_t h1 (get_z nq) /\
       state_inv_t h1 (get_x nq_p1) /\ state_inv_t h1 (get_z nq_p1) /\
      (let p2, p3 = P.add_and_double (fget_xz h0 q) (fget_xz h0 nq) (fget_xz h0 nq_p1) in
-      fget_xz h1 nq == p2 /\ fget_xz h1 nq_p1 == p3)))
+      fget_xz h1 nq == p2 /\ fget_xz h1 nq_p1 == p3))))
+
 [@ Meta.Attribute.specialize ]
-let point_add_and_double #s q p01_tmp1 tmp2 =
+let point_add_and_double #i q p01_tmp1 tmp2 =
+  [@inline_let]
+  let s, _ = i in
   let h0 = ST.get () in
   let nq : point s = sub p01_tmp1 0ul (2ul *! nlimb s) in
   let nq_p1 : point s = sub p01_tmp1 (2ul *! nlimb s) (2ul *! nlimb s) in
@@ -185,31 +197,36 @@ let point_add_and_double #s q p01_tmp1 tmp2 =
   let ab : felem2 s = sub tmp1 0ul (2ul *! nlimb s) in
   let dc : felem2 s = sub tmp1 (2ul *! nlimb s) (2ul *! nlimb s) in
 
-  fadd a x2 z2; // a = x2 + z2
-  fsub b x2 z2; // b = x2 - z2
+  fadd #i a x2 z2; // a = x2 + z2
+  fsub #i b x2 z2; // b = x2 - z2
 
-  point_add_and_double0 #s nq_p1 ab dc tmp2;
-  point_add_and_double1 #s nq nq_p1 tmp1 tmp2;
+  point_add_and_double0 #i nq_p1 ab dc tmp2;
+  point_add_and_double1 #i nq nq_p1 tmp1 tmp2;
   fmul z3 z3 x1 tmp2; // z3 = x1 * (da - cb) ^ 2
   S.lemma_add_and_double (fget_xz h0 q) (fget_xz h0 nq) (fget_xz h0 nq_p1)
 
 val point_double:
-    #s:field_spec
-  -> nq:point s
+    #i:index -> (
+  let s = fst i in
+  let p = snd i in
+    nq:point s
   -> tmp1:lbuffer (limb s) (4ul *! nlimb s)
   -> tmp2:felem_wide2 s
   -> Stack unit
     (requires fun h0 ->
-      (s = M64 ==> Vale.X64.CPU_Features_s.(adx_enabled /\ bmi2_enabled)) /\
+      p /\
       live h0 nq /\ live h0 tmp1 /\ live h0 tmp2 /\
       disjoint nq tmp1 /\ disjoint nq tmp2 /\ disjoint tmp1 tmp2 /\
       state_inv_t h0 (get_x nq) /\ state_inv_t h0 (get_z nq))
     (ensures  fun h0 _ h1 ->
       modifies (loc nq |+| loc tmp1 |+| loc tmp2) h0 h1 /\
       state_inv_t h1 (get_x nq) /\ state_inv_t h1 (get_z nq) /\
-      fget_xz h1 nq == P.double (fget_xz h0 nq))
+      fget_xz h1 nq == P.double (fget_xz h0 nq)))
+
 [@ Meta.Attribute.specialize ]
-let point_double #s nq tmp1 tmp2 =
+let point_double #i nq tmp1 tmp2 =
+  [@inline_let]
+  let s, _ = i in
   let x2 = sub nq 0ul (nlimb s) in
   let z2 = sub nq (nlimb s) (nlimb s) in
 
@@ -236,10 +253,10 @@ let point_double #s nq tmp1 tmp2 =
   //fsqr c b;     // c = bb = b^2
   fsqr2 dc ab tmp2;     // d|c = aa | bb
   copy_felem a c;                           // a = bb
-  fsub c d c;   // c = e = aa - bb
+  fsub #i c d c;   // c = e = aa - bb
   assert_norm (121665 < pow2 17);
-  fmul1 b c (u64 121665); // b = e * 121665
-  fadd b b d;   // b = (e * 121665) + aa
+  fmul1 #i b c (u64 121665); // b = e * 121665
+  fadd #i b b d;   // b = (e * 121665) + aa
 
   (* CAN RUN IN PARALLEL *)
   //fmul x2 d a;  // x2 = aa * bb
