code/curve25519/Hacl.Impl.Curve25519.Fields.Core.fsti
@@ -29,6 +29,35 @@ type field_spec =
   | M51
   | M64
 
+/// We allow the index to carry a global precondition that will be threaded
+/// throughout the call-graph.
+///
+/// A note on previous attempts... I tried to parameterize the call-graph over a
+/// [@ Specialize ] node that would contain a global precondition, possibly over
+/// a value of the field spec, e.g. ``assume val global_pre: field_spec ->
+/// Type`` then pair up the global pre with the index, i.e. ``type index =
+/// s:field_spec { global_pre s }``. The hope was to not have to manually carry
+/// the precondition everywhere, i.e. not augment all the call-graph with a
+/// requires clause. However, this is cumbersome, as this requires a lot of
+/// special treatment in the tactic, in order to rewrite ``let f #i:index`` into
+/// ``let f #s:field_spec (p: global_pre s)``, which would have been a
+/// significant complexity budget blowup. Also, some parts of the call-graph
+/// still wanted global_pre but not the index (because specialized on M64)...
+/// unpleasant and complicated.
+type index = field_spec & Type0
+
+/// In types, we can't do ``let s, p = i`` because it would block reduction and then we would have errors about things not having function types. However, if we do ``let s = fst i``, then ``fst`` being in Prims and *not* being marked as inline_for_extraction, reduction of the type, once applied to a constant, gets stuck. So, we redefine fst and snd.
+
+inline_for_extraction
+let fst p =
+  match p with
+  | x, y -> x
+
+inline_for_extraction
+let snd p =
+  match p with
+  | x, y -> y
+
 unfold noextract
 let limb (s:field_spec) =
   match s with
@@ -130,7 +159,7 @@ let fadd_fsub_pre (#s:field_spec) (h:mem) (f1:felem s) (f2:felem s): Type0 =
   | M51 ->
       f51_felem_fits h f1 (1, 2, 1, 1, 1) /\
       f51_felem_fits h f2 (1, 2, 1, 1, 1)
-  | M64 -> Vale.X64.CPU_Features_s.(adx_enabled /\ bmi2_enabled)
+  | M64 -> True
 
 let fadd_post (#s:field_spec) (h:mem) (out:felem s): Type0 =
   match s with
@@ -138,12 +167,15 @@ let fadd_post (#s:field_spec) (h:mem) (out:felem s): Type0 =
   | M64 -> True
 
 inline_for_extraction
-let fadd_t (s:field_spec) =
+let fadd_t (i: index) =
+  let s = fst i in
+  let p = snd i in
     out:felem s
   -> f1:felem s
   -> f2:felem s
   -> Stack unit
     (requires fun h ->
+      p /\
       live h out /\ live h f1 /\ live h f2 /\
       (disjoint out f1 \/ out == f1) /\
       (disjoint out f2 \/ out == f2) /\
@@ -153,7 +185,7 @@ let fadd_t (s:field_spec) =
       modifies (loc out) h0 h1 /\ fadd_post h1 out /\
       feval h1 out == P.fadd (feval h0 f1) (feval h0 f2))
 [@ Meta.Attribute.specialize]
-val fadd: #s:field_spec -> fadd_t s
+val fadd: #i:index -> fadd_t i
 
 let fsub_post (#s:field_spec) (h:mem) (out:felem s): Type0 =
   match s with
@@ -161,13 +193,15 @@ let fsub_post (#s:field_spec) (h:mem) (out:felem s): Type0 =
   | M64 -> True
 
 inline_for_extraction
-let fsub_t (s:field_spec) =
+let fsub_t (i: index) =
+  let s = fst i in
+  let p = snd i in
     out:felem s
   -> f1:felem s
   -> f2:felem s
   -> Stack unit
     (requires fun h ->
-      (s = M64 ==> Vale.X64.CPU_Features_s.(adx_enabled /\ bmi2_enabled)) /\
+      p /\
       live h out /\ live h f1 /\ live h f2 /\
       (disjoint out f1 \/ out == f1) /\
       (disjoint out f2 \/ out == f2) /\
@@ -177,14 +211,14 @@ let fsub_t (s:field_spec) =
       modifies (loc out) h0 h1 /\ fsub_post h1 out /\
       feval h1 out == P.fsub (feval h0 f1) (feval h0 f2))
 [@ Meta.Attribute.specialize ]
-val fsub: #s:field_spec -> fsub_t s
+val fsub: #i:index -> fsub_t i
 
 let fmul_pre (#s:field_spec) (h:mem) (f1:felem s) (f2:felem s): Type0 =
   match s with
   | M51 ->
       f51_felem_fits h f1 (9, 10, 9, 9, 9) /\
       f51_felem_fits h f2 (9, 10, 9, 9, 9)
-  | M64 -> Vale.X64.CPU_Features_s.(adx_enabled /\ bmi2_enabled)
+  | M64 -> True
 
 let fmul_disjoint (#s:field_spec) (out f1 f2:felem s) (tmp:felem_wide2 s): Type0 =
   match s with
@@ -204,13 +238,16 @@ let state_inv_t (#s:field_spec) (h:mem) (f:felem s): Type0 =
   | M64 -> True
 
 inline_for_extraction
-let fmul_t (s:field_spec) =
+let fmul_t (i: index) =
+  let s = fst i in
+  let p = snd i in
     out:felem s
   -> f1:felem s
   -> f2:felem s
   -> tmp:felem_wide2 s
   -> Stack unit
     (requires fun h ->
+      p /\
       live h out /\ live h f1 /\ live h f2 /\ live h tmp /\
       fmul_disjoint out f1 f2 tmp /\
       fmul_pre h f1 f2)
@@ -218,7 +255,7 @@ let fmul_t (s:field_spec) =
       modifies (loc out |+| loc tmp) h0 h1 /\ state_inv_t h1 out /\
       feval h1 out == P.fmul (feval h0 f1) (feval h0 f2))
 [@ Meta.Attribute.specialize ]
-val fmul: #s:field_spec -> fmul_t s
+val fmul: #i:index -> fmul_t i
 
 let fmul2_pre (#s:field_spec) (h:mem) (f1:felem2 s) (f2:felem2 s): Type0 =
   match s with
@@ -231,7 +268,7 @@ let fmul2_pre (#s:field_spec) (h:mem) (f1:felem2 s) (f2:felem2 s): Type0 =
       f51_felem_fits h f11 (9, 10, 9, 9, 9) /\
       f51_felem_fits h f20 (9, 10, 9, 9, 9) /\
       f51_felem_fits h f21 (9, 10, 9, 9, 9)
-  | M64 -> Vale.X64.CPU_Features_s.(adx_enabled /\ bmi2_enabled)
+  | M64 -> True
 
 let fmul2_fsqr2_post (#s:field_spec) (h:mem) (out:felem2 s): Type0 =
   match s with
@@ -243,13 +280,16 @@ let fmul2_fsqr2_post (#s:field_spec) (h:mem) (out:felem2 s): Type0 =
   | M64 -> True
 
 inline_for_extraction
-let fmul2_t (s:field_spec) =
+let fmul2_t (i: index) =
+  let s = fst i in
+  let p = snd i in
     out:felem2 s
   -> f1:felem2 s
   -> f2:felem2 s
   -> tmp:felem_wide2 s
   -> Stack unit
     (requires fun h ->
+      p /\
       live h out /\ live h f1 /\ live h f2 /\ live h tmp /\
       (disjoint out f1 \/ out == f1) /\
       (disjoint out f2 \/ out == f2) /\
@@ -270,20 +310,23 @@ let fmul2_t (s:field_spec) =
       feval h1 out1 == P.fmul (feval h0 f11) (feval h0 f21)))
 
 [@ Meta.Attribute.specialize ]
-val fmul2: #s:field_spec -> fmul2_t s
+val fmul2: #i:index -> fmul2_t i
 
 let fmul1_pre (#s:field_spec) (h:mem) (f1:felem s) (f2:uint64): Type0 =
   match s with
   | M51 -> f51_felem_fits h f1 (9, 10, 9, 9, 9) /\ f51_felem_fits1 f2 1
-  | M64 -> v f2 < pow2 17 /\ Vale.X64.CPU_Features_s.(adx_enabled /\ bmi2_enabled)
+  | M64 -> v f2 < pow2 17
 
 inline_for_extraction
-let fmul1_t (s:field_spec) =
+let fmul1_t (i: index) =
+  let s = fst i in
+  let p = snd i in
     out:felem s
   -> f1:felem s
   -> f2:uint64
   -> Stack unit
     (requires fun h ->
+      p /\
       live h out /\ live h f1 /\
       (disjoint out f1 \/ out == f1) /\
       fmul1_pre h f1 f2)
@@ -293,12 +336,12 @@ let fmul1_t (s:field_spec) =
 //     feval h1 out == (feval h0 f1 * v f2) % P.prime)
 
 [@ Meta.Attribute.specialize ]
-val fmul1: #s:field_spec -> fmul1_t s
+val fmul1: #i:index -> fmul1_t i
 
 let fsqr_pre (#s:field_spec) (h:mem) (f:felem s): Type0 =
   match s with
   | M51 -> f51_felem_fits h f (9, 10, 9, 9, 9)
-  | M64 -> Vale.X64.CPU_Features_s.(adx_enabled /\ bmi2_enabled)
+  | M64 -> True
 
 let fsqr_disjoint (#s:field_spec) (out f1:felem s) (tmp:felem_wide s): Type0 =
   match s with
@@ -309,12 +352,15 @@ let fsqr_disjoint (#s:field_spec) (out f1:felem s) (tmp:felem_wide s): Type0 =
       disjoint tmp f1
 
 inline_for_extraction
-let fsqr_t (s:field_spec) =
+let fsqr_t (i: index) =
+  let s = fst i in
+  let p = snd i in
     out:felem s
   -> f1:felem s
   -> tmp:felem_wide s
   -> Stack unit
     (requires fun h ->
+      p /\
       live h out /\ live h f1 /\ live h tmp /\
       fsqr_disjoint out f1 tmp /\
       fsqr_pre h f1)
@@ -324,7 +370,7 @@ let fsqr_t (s:field_spec) =
       feval h1 out == P.fmul (feval h0 f1) (feval h0 f1))
 
 [@ Meta.Attribute.specialize ]
-val fsqr: #s:field_spec -> fsqr_t s
+val fsqr: #i:index -> fsqr_t i
 
 let fsqr2_pre (#s:field_spec) (h:mem) (f:felem2 s): Type0 =
   match s with
@@ -333,15 +379,18 @@ let fsqr2_pre (#s:field_spec) (h:mem) (f:felem2 s): Type0 =
       let f2 = gsub f 5ul 5ul in
       f51_felem_fits h f1 (9, 10, 9, 9, 9) /\
       f51_felem_fits h f2 (9, 10, 9, 9, 9)
-  | M64 -> Vale.X64.CPU_Features_s.(adx_enabled /\ bmi2_enabled)
+  | M64 -> True
 
 inline_for_extraction
-let fsqr2_t (s:field_spec) =
+let fsqr2_t (i: index) =
+  let s = fst i in
+  let p = snd i in
     out:felem2 s
   -> f:felem2 s
   -> tmp:felem_wide2 s
   -> Stack unit
     (requires fun h ->
+      p /\
       live h out /\ live h f /\ live h tmp /\
       (disjoint out f \/ out == f) /\
       (disjoint out tmp \/ out == tmp) /\
@@ -357,16 +406,18 @@ let fsqr2_t (s:field_spec) =
       feval h1 out2 == P.fmul (feval h0 f2) (feval h0 f2)))
 
 [@ Meta.Attribute.specialize ]
-val fsqr2: #s:field_spec -> fsqr2_t s
+val fsqr2: #i:index -> fsqr2_t i
 
 inline_for_extraction
-let cswap2_t (s:field_spec) =
+let cswap2_t (i: index) =
+  let s = fst i in
+  let p = snd i in
     bit:uint64{v bit <= 1}
   -> p1:felem2 s
   -> p2:felem2 s
   -> Stack unit
     (requires fun h0 ->
-      (s = M64 ==> Vale.X64.CPU_Features_s.(adx_enabled /\ bmi2_enabled)) /\
+      p /\
       live h0 p1 /\ live h0 p2 /\
       (disjoint p1 p2 \/ p1 == p2))
     (ensures  fun h0 _ h1 ->
@@ -375,20 +426,23 @@ let cswap2_t (s:field_spec) =
       (v bit == 0 ==> as_seq h1 p1 == as_seq h0 p1 /\ as_seq h1 p2 == as_seq h0 p2))
 
 [@ Meta.Attribute.specialize ]
-val cswap2: #s:field_spec -> cswap2_t s
+val cswap2: #i:index -> cswap2_t i
 
 /// Field64-specific core operations
 /// --------------------------------
 
 inline_for_extraction
-let add1_t = out:felem M64 -> f1:felem M64 -> f2:uint64
+let add1_t (i: index) =
+  let s = fst i in
+  let p = snd i in
+  out:felem s -> f1:felem s -> f2:uint64
   -> Stack uint64
     (requires fun h ->
-      Vale.X64.CPU_Features_s.(adx_enabled /\ bmi2_enabled) /\
+      s == M64 /\ p /\
       live h f1 /\ live h out /\
       (disjoint out f1 \/ out == f1))
     (ensures  fun h0 c h1 ->
       modifies (loc out) h0 h1 /\
       as_nat h1 out + v c * pow2 256 == as_nat h0 f1 + v f2)
 [@ CInline Meta.Attribute.specialize ]
-val add1: add1_t
+val add1: #i:index -> add1_t i
