code/curve25519/Hacl.Curve25519_64.fsti
@@ -3,6 +3,6 @@ module Hacl.Curve25519_64
 open Hacl.Impl.Curve25519.Generic
 open Hacl.Impl.Curve25519.Fields
 
-val scalarmult: scalarmult_st M64
-val secret_to_public: secret_to_public_st M64
-val ecdh: ecdh_st M64
+val scalarmult: scalarmult_st (M64, Vale.X64.CPU_Features_s.(adx_enabled /\ bmi2_enabled))
+val secret_to_public: secret_to_public_st (M64, Vale.X64.CPU_Features_s.(adx_enabled /\ bmi2_enabled))
+val ecdh: ecdh_st (M64, Vale.X64.CPU_Features_s.(adx_enabled /\ bmi2_enabled))
