code/curve25519/Hacl.Impl.Curve25519.Field64.Local.fsti
@@ -6,12 +6,16 @@ open Hacl.Impl.Curve25519.Fields.Core
 /// and removing the fst from the include path because this leaves invalid build
 /// artifacts in the shared obj directory.
 
-val add1: add1_t
-val fadd: fadd_t M64
-val fsub: fsub_t M64
-val fmul: fmul_t M64
-val fmul2: fmul2_t M64
-val fmul1: fmul1_t M64
-val fsqr: fsqr_t M64
-val fsqr2: fsqr2_t M64
-val cswap2: cswap2_t M64
+// Note: this doesn't work and the types don't reduce.
+// inline_for_extraction
+// let i = M64, True
+
+val add1: add1_t (M64, True)
+val fadd: fadd_t (M64, True)
+val fsub: fsub_t (M64, True)
+val fmul: fmul_t (M64, True)
+val fmul2: fmul2_t (M64, True)
+val fmul1: fmul1_t (M64, True)
+val fsqr: fsqr_t (M64, True)
+val fsqr2: fsqr2_t (M64, True)
+val cswap2: cswap2_t (M64, True)
